veric/extension_proof.v
@@ -20,7 +20,7 @@ intros ge n; induction n; auto.
 intros  ora c m; simpl; intros H1.
 destruct (at_external CS c).
 destruct p; destruct p.
-destruct (safely_halted CS ge c).
+destruct (safely_halted CS c).
 auto.
 destruct H1 as [x [H1 H2]].
 if_tac in H1.
@@ -28,7 +28,7 @@ elimtype False; apply H1.
 exists x; split; auto.
 intros ret m' z' H3; destruct (H2 ret m' z' H3) as [c' [H4 H5]].
 exists c'; split; auto.
-destruct (safely_halted CS ge c); auto.
+destruct (safely_halted CS c); auto.
 destruct H1 as [c' [m' [H1 H2]]].
 exists c'; exists m'; split; auto.
 Qed.
@@ -39,6 +39,7 @@ Module ExtensionSafety. Section ExtensionSafety.
  Variables
   (G: Type) (** global environments *)
   (xT: Type) (** corestates of extended semantics *)
+  (gT: nat -> Type) (** global environments of the core semantics *)
   (cT: nat -> Type) (** corestates of core semantics *)
   (M: Type) (** memories *)
   (D: Type) (** initialization data *)
@@ -47,12 +48,12 @@ Module ExtensionSafety. Section ExtensionSafety.
   (Zext: Type) (** portion of Z external to extension *)
 
   (esem: CoreSemantics G xT M D) (** extended semantics *)
-  (csem: forall i:nat, option (CoreSemantics G (cT i) M D)) (** a set of core semantics *)
+  (csem: forall i:nat, option (CoreSemantics (gT i) (cT i) M D)) (** a set of core semantics *)
 
   (csig: ext_sig M Z) (** client signature *)
   (esig: ext_sig M Zext) (** extension signature *)
   (handled: list AST.external_function) (** functions handled by this extension *)
-  (E: Extension.Sig cT Zint esem csem csig esig handled). 
+  (E: Extension.Sig gT cT Zint esem csem csig esig handled). 
 
 Import SafetyInvariant.
 Import TruePropCoercion.
@@ -83,14 +84,14 @@ Notation runnable_false := E.(Extension.runnable_false).
 Program Definition ExtensionSafety: EXTENSION_SAFETY.Sig E.
 Proof.
 constructor.
-inversion 1; subst; intros ge n; induction n.
+inversion 1; subst; intros n; induction n.
 intros s m z H1; simpl; auto.
 intros s m z H1.
 simpl; case_eq (at_external esem s).
 
 (*CASE 1: at_external OUTER = Some _; i.e. _really_ at_external*) 
 intros [[ef sig] args] AT_EXT.
-destruct (at_external_halted_excl esem ge s) as [H2|H2].
+destruct (at_external_halted_excl esem s) as [H2|H2].
 rewrite AT_EXT in H2; congruence.
 simpl; rewrite H2.
 destruct (at_extern_call s ef sig args AT_EXT) as [CS [c [[H3 H4] H5]]].
@@ -98,7 +99,7 @@ generalize H1 as H1'; intro.
 specialize (H1 (ACTIVE s) CS c H3 H4).
 simpl in H1.
 rewrite H5 in H1.
-destruct (at_external_halted_excl CS ge c) as [H6|H6].
+destruct (at_external_halted_excl CS c) as [H6|H6].
 rewrite H6 in H5; congruence.
 rewrite H6 in H1; clear H6.
 destruct H1 as [x H1].
@@ -169,15 +170,15 @@ destruct H19 as [H21 H22]; auto.
 
 (*CASE 2: at_external OUTER = None; i.e., inner corestep or handled function*)
 intros H2.
-case_eq (safely_halted esem ge s); auto.
-case_eq (RUNNABLE ge s).
+case_eq (safely_halted esem s); auto.
+case_eq (RUNNABLE s).
 (*active thread i is runnable*)
 intros RUN.
 destruct (active_csem s) as [CS CSEM].
 destruct (active_proj_core s) as [c PROJECT].
-destruct (core_prog ge n (s \o z) s m c CS H1 RUN)
+destruct (core_prog n (s \o z) s m c CS H1 RUN)
  as [c' [s' [m' [CORESTEP_C [CORESTEP_T ?]]]]]; auto.
-generalize (core_pres ge n z s c m CS s' c' m' H1)
+generalize (core_pres n z s c m CS s' c' m' H1)
  as INV'; auto.
 intros Hsafehalt.
 exists s'; exists m'; split; [auto|].
@@ -187,13 +188,13 @@ eauto.
 intros RUN.
 destruct (active_csem s) as [CS CSEM].
 destruct (active_proj_core s) as [c PROJECT].
-destruct (handled_prog ge n z s m H1 RUN H2)
+destruct (handled_prog n z s m H1 RUN H2)
  as [[s' [m' [CORESTEP_T CORES_PRES]]]|[rv SAFELY_HALTED]].
 2: intros CONTRA; rewrite CONTRA in SAFELY_HALTED; congruence.
 exists s'; exists m'.
 split; auto.
 eapply IHn.
-destruct (runnable_false ge s RUN CSEM PROJECT) 
+destruct (runnable_false s RUN CSEM PROJECT) 
  as [SAFELY_HALTED|[ef [sig [args AT_EXT]]]].
 
 (*subcase A of no runnable thread: safely halted*)
@@ -203,24 +204,24 @@ case_eq (eq_nat_dec i j).
 (*i=j*)
 intros Heq _.
 subst j.
-destruct (core_exists ge i s m s' m' CORESTEP_T PROJECTj)
+destruct (core_exists (Extension.ge E) i s m s' m' CORESTEP_T PROJECTj)
  as [c0 PROJECT0].
 rewrite PROJECT in PROJECT0; inversion PROJECT0; subst.
 rewrite CSEM in CSEMj; inversion CSEMj; rename H4 into H3; rewrite <-H3 in *.
 specialize (H1 i CS c0 CSEM PROJECT).
 simpl in H1. 
 destruct SAFELY_HALTED as [rv SAFELY_HALTED].
-destruct (@at_external_halted_excl G (cT i) M D CS ge c0) as [H4|H4]; 
+destruct (@at_external_halted_excl (gT i) (cT i) M D CS c0) as [H4|H4]; 
  [|congruence].
 destruct n; simpl; auto.
-destruct (safely_halted_halted ge s m s' m' i CS c0 rv) as [H6 H7]; auto.
+destruct (safely_halted_halted s m s' m' i CS c0 rv) as [H6 H7]; auto.
 rewrite H7 in PROJECTj; inversion PROJECTj; subst.
 rewrite H4, SAFELY_HALTED; auto.
 (*i<>j*)
 intros Hneq _.
 destruct (CORES_PRES i c CS) as [c' [[_ PROJ'] H5]]. 
 split; auto.
-specialize (handled_rest ge s m s' m' c CS).
+specialize (handled_rest s m s' m' c CS).
 hnf in handled_rest.
 spec handled_rest; auto.
 spec handled_rest; auto.
@@ -229,7 +230,7 @@ spec handled_rest; auto.
 destruct (handled_rest j CSj cj Hneq) as [H6 H7].
 eapply H7 with (z:=z); eauto.
 eapply H1; eauto.
-destruct (core_exists ge j s m s' m' CORESTEP_T PROJECTj)
+destruct (core_exists (Extension.ge E) j s m s' m' CORESTEP_T PROJECTj)
  as [c0 PROJECT0].
 specialize (H1 j CSj c0 CSEMj PROJECT0).
 destruct H6 as [H8 H9].
@@ -243,7 +244,7 @@ case_eq (eq_nat_dec i j).
 (*i=j*)
 intros Heq _.
 subst j.
-destruct (core_exists ge i s m s' m' CORESTEP_T PROJECTj)
+destruct (core_exists (Extension.ge E) i s m s' m' CORESTEP_T PROJECTj)
  as [c0 PROJECT0].
 rewrite PROJECT in PROJECT0; inversion PROJECT0; subst.
 generalize CSEMj as CSEMj'; intro.
@@ -251,12 +252,12 @@ rewrite CSEM in CSEMj; inversion CSEMj; rename H4 into H3; rewrite <-H3 in *.
 specialize (H1 i CS c0 CSEM PROJECT).
 simpl in H1. 
 rewrite AT_EXT in H1.
-remember (safely_halted CS ge c0) as SAFELY_HALTED.
+remember (safely_halted CS c0) as SAFELY_HALTED.
 destruct SAFELY_HALTED. 
 solve[destruct ef; elimtype False; auto].
 destruct H1 as [x H1].
 destruct H1 as [PRE POST].
-specialize (handled_pres ge s z m c0 s' m' cj CS ef sig args
+specialize (handled_pres s z m c0 s' m' cj CS ef sig args
   (ext_spec_pre csig ef)
   (ext_spec_post csig ef) x).
 (*rewrite Heq in handled_pres.*)
@@ -293,7 +294,7 @@ generalize (after_at_external_excl CS ret c0 c' AFTER_EXT); intros AT_EXT'.
 clear - PRE POST POST' AT_EXT' AFTER_EXT H4 H5 H6 HeqSAFELY_HALTED.
 destruct n; simpl; auto.
 rewrite AT_EXT'.
-case_eq (safely_halted CS ge c'); auto.
+case_eq (safely_halted CS c'); auto.
 destruct (POST ret m' (s' \o z) POST') as [c'' [AFTER_EXT' SAFEN]].
 unfold i in AFTER_EXT'.
 rewrite AFTER_EXT in AFTER_EXT'; inversion AFTER_EXT'; subst.
@@ -306,7 +307,7 @@ exists c3; exists m''; split; auto.
 intros Hneq _.
 destruct (CORES_PRES i c CS) as [c' [[_ PROJ'] H5]]. 
 split; auto.
-specialize (handled_rest ge s m s' m' c CS).
+specialize (handled_rest s m s' m' c CS).
 hnf in handled_rest.
 spec handled_rest; auto.
 spec handled_rest; auto.
@@ -316,7 +317,7 @@ spec handled_rest; auto.
 destruct (handled_rest j CSj cj Hneq) as [H6 H7].
 eapply H7 with (z:=z); eauto.
 eapply H1; eauto.
-destruct (core_exists ge j s m s' m' CORESTEP_T PROJECTj)
+destruct (core_exists (Extension.ge E) j s m s' m' CORESTEP_T PROJECTj)
  as [c0 PROJECT0].
 specialize (H1 j CSj c0 CSEMj PROJECT0).
 destruct H6 as [H8 H9].
@@ -328,24 +329,24 @@ End ExtensionSafety. End ExtensionSafety.
 
 Section CoreCompatibleLemmas.
 Variables 
-  (G xT M D Z Zint Zext: Type) (cT: nat -> Type)
-  (esem: CoreSemantics G xT M D) 
-  (csem: forall i:nat, option (CoreSemantics G (cT i) M D))
-  (csig: ext_sig M Z)
-  (esig: ext_sig M Zext)
-  (handled: list AST.external_function)
-  (E: Extension.Sig cT Zint esem csem csig esig handled).
+ (G xT M D Z Zint Zext: Type) (gT: nat -> Type) (cT: nat -> Type)
+ (esem: CoreSemantics G xT M D) 
+ (csem: forall i:nat, option (CoreSemantics (gT i) (cT i) M D))
+ (csig: ext_sig M Z)
+ (esig: ext_sig M Zext)
+ (handled: list AST.external_function)
+ (E: Extension.Sig gT cT Zint esem csem csig esig handled).
 
 Variable Hcore_compatible: core_compatible E.
 
 Import Extension.
 
 Lemma corestep_step: 
-  forall ge s (c: cT (active E s)) m c' m' CS,
+  forall s (c: cT (active E s)) m c' m' CS,
   csem (active E s) = Some CS -> 
   proj_core E (active E s) s = Some c -> 
-  corestep CS ge c m c' m' -> 
-  exists s', corestep esem ge s m s' m' /\
+  corestep CS (genv_map E (active E s)) c m c' m' -> 
+  exists s', corestep esem (Extension.ge E) s m s' m' /\
     active E s = active E s' /\ proj_core E (active E s) s' = Some c'.
 Proof.
 intros.
@@ -354,21 +355,20 @@ generalize H1 as H1'; intro.
 eapply corestep_prog in H1; eauto.
 destruct H1 as [s' H1].
 exists s'.
-split; auto. 
-eapply corestep_pres; eauto.
+split; eauto. 
 Qed.
 
 Lemma corestep_stepN: 
-  forall n ge s (c: cT (active E s)) m c' m' CS,
+  forall n s (c: cT (active E s)) m c' m' CS,
   csem (active E s) = Some CS -> 
   proj_core E (active E s) s = Some c -> 
-  corestepN CS ge n c m c' m' -> 
-  exists s', corestepN esem ge n s m s' m' /\ 
+  corestepN CS (genv_map E (active E s)) n c m c' m' -> 
+  exists s', corestepN esem (Extension.ge E) n s m s' m' /\ 
     active E s = active E s' /\ proj_core E (active E s) s' = Some c'.
 Proof.
 inv Hcore_compatible.
 generalize corestep_step; intro H1.
-intros n ge.
+intros n.
 induction n; auto.
 intros.
 inv H2.
@@ -386,17 +386,17 @@ destruct (IHn s2 c2 m2 c' m' CS) as [s' [H10 [H11 H13]]]; auto.
 exists s'.
 split3.
 simpl.
-exists s2; exists m2; split; auto.
+exists s2; exists m2; split; eauto.
 auto.
 auto.
 Qed.
 
 Lemma corestep_step_star: 
-  forall ge s (c: cT (active E s)) m c' m' CS,
+  forall s (c: cT (active E s)) m c' m' CS,
   csem (active E s) = Some CS -> 
   proj_core E (active E s) s = Some c -> 
-  corestep_star CS ge c m c' m' -> 
-  exists s', corestep_star esem ge s m s' m' /\ 
+  corestep_star CS (genv_map E (active E s)) c m c' m' -> 
+  exists s', corestep_star esem (Extension.ge E) s m s' m' /\ 
     active E s = active E s' /\ proj_core E (active E s) s' = Some c'.
 Proof.
 intros.
@@ -405,15 +405,15 @@ eapply corestep_stepN in H1; eauto.
 destruct H1 as [s' [H1 [H2 H4]]].
 exists s'.
 split3; auto.
-exists n; auto.
+exists n; eauto.
 Qed.
 
 Lemma corestep_step_plus: 
-  forall ge s (c: cT (active E s)) m c' m' CS,
+  forall s (c: cT (active E s)) m c' m' CS,
   csem (active E s) = Some CS -> 
   proj_core E (active E s) s = Some c -> 
-  corestep_plus CS ge c m c' m' -> 
-  exists s', corestep_plus esem ge s m s' m' /\ 
+  corestep_plus CS (genv_map E (active E s)) c m c' m' -> 
+  exists s', corestep_plus esem (Extension.ge E) s m s' m' /\ 
     active E s = active E s' /\ proj_core E (active E s) s' = Some c'.
 Proof.
 intros.
@@ -422,7 +422,7 @@ eapply corestep_stepN in H1; eauto.
 destruct H1 as [s' [H1 [H2 H4]]].
 exists s'.
 split3; auto.
-exists n; auto.
+exists n; eauto.
 Qed.
 
 End CoreCompatibleLemmas.
@@ -431,6 +431,7 @@ Module ExtendedSimulations. Section ExtendedSimulations.
  Variables
   (F V: Type) (** global environments *)
   (xS xT: Type) (** corestates of source and target extended semantics *)
+  (fS fT vS vT: nat -> Type) (** global environments of core semantics *)
   (cS cT: nat -> Type) (** corestates of source and target core semantics *)
   (dS dT: Type) (** initialization data *)
   (Z: Type) (** external states *)
@@ -438,22 +439,40 @@ Module ExtendedSimulations. Section ExtendedSimulations.
   (Zext: Type) (** portion of Z external to extension *)
   (esemS: CoreSemantics (Genv.t F V) xS mem dS) (** extended source semantics *)
   (esemT: CoreSemantics (Genv.t F V) xT mem dT) (** extended target semantics *)
-  (csemS: forall i:nat, CoreSemantics (Genv.t F V) (cS i) mem dS) (** a set of core semantics *)
-  (csemT: forall i:nat, CoreSemantics (Genv.t F V) (cT i) mem dT) (** a set of core semantics *)
+  (csemS: forall i:nat, CoreSemantics (Genv.t (fS i) (vS i)) (cS i) mem dS) (** a set of core semantics *)
+  (csemT: forall i:nat, CoreSemantics (Genv.t (fT i) (vT i)) (cT i) mem dT) (** a set of core semantics *)
   (csig: ext_sig mem Z) (** client signature *)
   (esig: ext_sig mem Zext) (** extension signature *)
   (handled: list AST.external_function). (** functions handled by this extension *)
 
- Variable (E_S: Extension.Sig cS Zint esemS (fun i:nat => Some (csemS i)) csig esig handled).
- Variable (E_T: Extension.Sig cT Zint esemT (fun i:nat => Some (csemT i)) csig esig handled).
+ Variable (E_S: Extension.Sig (fun i => Genv.t (fS i) (vS i)) cS Zint esemS 
+                  (fun i:nat => Some (csemS i)) csig esig handled).
+ Variable (E_T: Extension.Sig (fun i => Genv.t (fT i) (vT i)) cT Zint esemT 
+                  (fun i:nat => Some (csemT i)) csig esig handled).
 
- Variable ge: Genv.t F V.
  Variable entry_points: list (val*val*signature).
+
+ Notation GENV_MAP := (Extension.genv_map).
+ Notation PROJ_CORE := (Extension.proj_core).
+ Infix "\o" := (Extension.zmult) (at level 66, left associativity). 
+ Notation ACTIVE := (Extension.active).
+ Notation RUNNABLE := (Extension.runnable).
+ Notation "'CORE' i 'is' ( CS , c ) 'in' s" := 
+   (csem i = Some CS /\ PROJ_CORE i s = Some c)
+   (at level 66, no associativity, only parsing).
+ Notation core_exists := (Extension.core_exists).
+ Notation active_csem := (Extension.active_csem).
+ Notation active_proj_core := (Extension.active_proj_core).
+ Notation notat_external_handled := (Extension.notat_external_handled).
+ Notation at_external_not_handled := (Extension.at_external_not_handled).
+ Notation ext_upd_at_external := (Extension.ext_upd_at_external).
+ Notation runnable_false := (Extension.runnable_false).
 
  Import Sim_inj.
 
  Variable core_simulations: forall i:nat, 
-   Forward_simulation_inject dS dT (csemS i) (csemT i) ge ge entry_points.
+   Forward_simulation_inject dS dT (csemS i) (csemT i) 
+     (GENV_MAP E_S i) (GENV_MAP E_T i) entry_points.
 
  Variable threads_max: nat.
 
@@ -523,24 +542,9 @@ Module ExtendedSimulations. Section ExtendedSimulations.
  elimtype False; omega.
  Qed.
 
- Notation PROJ_CORE := (Extension.proj_core).
- Infix "\o" := (Extension.zmult) (at level 66, left associativity). 
- Notation ACTIVE := (Extension.active).
- Notation RUNNABLE := (Extension.runnable).
- Notation "'CORE' i 'is' ( CS , c ) 'in' s" := 
-   (csem i = Some CS /\ PROJ_CORE i s = Some c)
-   (at level 66, no associativity, only parsing).
- Notation core_exists := (Extension.core_exists).
- Notation active_csem := (Extension.active_csem).
- Notation active_proj_core := (Extension.active_proj_core).
- Notation notat_external_handled := (Extension.notat_external_handled).
- Notation at_external_not_handled := (Extension.at_external_not_handled).
- Notation ext_upd_at_external := (Extension.ext_upd_at_external).
- Notation runnable_false := (Extension.runnable_false).
-
  Definition match_states (cd: core_datas) (j: meminj) (s1: xS) m1 (s2: xT) m2 :=
    ACTIVE E_S s1=ACTIVE E_T s2 /\
-   RUNNABLE E_S ge s1=RUNNABLE E_T ge s2 /\
+   RUNNABLE E_S s1=RUNNABLE E_T s2 /\
    forall i c1, PROJ_CORE E_S i s1 = Some c1 -> 
      exists c2, PROJ_CORE E_T i s2 = Some c2 /\ 
        match_state (core_simulations i) (cd i) j c1 m1 c2 m2.
@@ -555,69 +559,69 @@ Module ExtendedSimulations. Section ExtendedSimulations.
     ACTIVE E_S s1 <> i -> 
     match_states cd j s1 m1 s2 m2 -> 
     Mem.inject j m1 m2 -> 
-    meminj_preserves_globals (genv2blocks ge) j -> 
+    meminj_preserves_globals (genv2blocks (Extension.ge E_S)) j -> 
     inject_incr j j' -> 
     Events.inject_separated j j' m1 m2 -> 
-    corestep (csemS (ACTIVE E_S s1)) ge c1 m1 c1' m1' -> 
-    corestepN (csemT (ACTIVE E_S s1)) ge n c2 m2 c2' m2' -> 
+    corestep (csemS (ACTIVE E_S s1)) (GENV_MAP E_S (ACTIVE E_S s1)) c1 m1 c1' m1' -> 
+    corestepN (csemT (ACTIVE E_S s1)) (GENV_MAP E_T (ACTIVE E_S s1)) n c2 m2 c2' m2' -> 
     match_state (core_simulations (ACTIVE E_S s1)) cd' j' c1' m1' c2' m2' -> 
     match_state (core_simulations i) (cd i) j' d1 m1' d2 m2')
 
   (corestep_runnable: forall s1 c1 m1 c1' m1' s1' s2 c2 m2 c2' m2' s2' n,
     PROJ_CORE E_S (ACTIVE E_S s1) s1 = Some c1 -> 
     PROJ_CORE E_T (ACTIVE E_S s1) s2 = Some c2 -> 
-    RUNNABLE E_S ge s1=RUNNABLE E_T ge s2 -> 
-    corestep (csemS (ACTIVE E_S s1)) ge c1 m1 c1' m1' -> 
-    corestepN (csemT (ACTIVE E_S s1)) ge n c2 m2 c2' m2' -> 
-    corestep esemS ge s1 m1 s1' m1' -> 
-    corestepN esemT ge n s2 m2 s2' m2' -> 
-    RUNNABLE E_S ge s1'=RUNNABLE E_T ge s2')
+    RUNNABLE E_S s1=RUNNABLE E_T s2 -> 
+    corestep (csemS (ACTIVE E_S s1)) (GENV_MAP E_S (ACTIVE E_S s1)) c1 m1 c1' m1' -> 
+    corestepN (csemT (ACTIVE E_S s1)) (GENV_MAP E_T (ACTIVE E_S s1)) n c2 m2 c2' m2' -> 
+    corestep esemS (Extension.ge E_S) s1 m1 s1' m1' -> 
+    corestepN esemT (Extension.ge E_T) n s2 m2 s2' m2' -> 
+    RUNNABLE E_S s1'=RUNNABLE E_T s2')     
 
   (extension_diagram: forall s1 m1 s1' m1' s2 c1 c2 m2 ef sig args1 args2 cd j,
-    RUNNABLE E_S ge s1=false -> RUNNABLE E_T ge s2=false -> 
+    RUNNABLE E_S s1=false -> RUNNABLE E_T s2=false -> 
     PROJ_CORE E_S (ACTIVE E_S s1) s1 = Some c1 -> 
     PROJ_CORE E_T (ACTIVE E_S s1) s2 = Some c2 -> 
     at_external (csemS (ACTIVE E_S s1)) c1 = Some (ef, sig, args1) -> 
     at_external (csemT (ACTIVE E_S s1)) c2 = Some (ef, sig, args2) -> 
     match_states cd j s1 m1 s2 m2 -> 
     Mem.inject j m1 m2 -> 
-    Events.meminj_preserves_globals ge j -> 
+    Events.meminj_preserves_globals (Extension.ge E_S) j -> 
     Forall2 (val_inject j) args1 args2 -> 
     Forall2 Val.has_type args2 (sig_args sig) -> 
-    corestep esemS ge s1 m1 s1' m1' -> 
+    corestep esemS (Extension.ge E_S) s1 m1 s1' m1' -> 
     exists s2', exists m2', exists cd', exists j',
       inject_incr j j' /\
       Events.inject_separated j j' m1 m2 /\
       match_states cd' j' s1' m1' s2' m2' /\
-      corestep esemT ge s2 m2 s2' m2')
+      corestep esemT (Extension.ge E_T) s2 m2 s2' m2')
 
   (at_external_match: forall s1 m1 s2 c1 c2 m2 ef sig args1 args2 cd j,
     ACTIVE E_S s1=ACTIVE E_T s2 -> 
-    RUNNABLE E_S ge s1=RUNNABLE E_T ge s2 -> 
+    RUNNABLE E_S s1=RUNNABLE E_T s2 -> 
     PROJ_CORE E_S (ACTIVE E_S s1) s1 = Some c1 -> 
     PROJ_CORE E_T (ACTIVE E_S s1) s2 = Some c2 -> 
     at_external esemS s1 = Some (ef, sig, args1) -> 
     at_external (csemS (ACTIVE E_S s1)) c1 = Some (ef, sig, args1) -> 
     match_state (core_simulations (ACTIVE E_S s1)) cd j c1 m1 c2 m2 -> 
     Mem.inject j m1 m2 -> 
-    Events.meminj_preserves_globals ge j -> 
+    Events.meminj_preserves_globals (Extension.ge E_S) j -> 
     Forall2 (val_inject j) args1 args2 -> 
     Forall2 Val.has_type args2 (sig_args sig) -> 
     at_external (csemT (ACTIVE E_S s1)) c2 = Some (ef, sig, args2) -> 
     at_external esemT s2 = Some (ef, sig, args2))
-
-  (after_external_runnable: forall ge s1 m1 s2 m2 retv1 retv2 s1' s2' cd j,
-    RUNNABLE E_S ge s1=RUNNABLE E_T ge s2 -> 
+  
+  (after_external_runnable: forall s1 m1 s2 m2 retv1 retv2 s1' s2' cd j,
+    RUNNABLE E_S s1=RUNNABLE E_T s2 -> 
     match_states cd j s1 m1 s2 m2 -> 
     after_external esemS retv1 s1 = Some s1' -> 
     after_external esemT retv2 s2 = Some s2' ->     
-    RUNNABLE E_S ge s1'=RUNNABLE E_T ge s2')
+    RUNNABLE E_S s1'=RUNNABLE E_T s2')
 
   (after_external_diagram: 
     forall i d1 s1 m1 d2 s2 m2 s1' m1' s2' m2' ef sig args1 retv1 retv2 cd j j',
     match_state (core_simulations i) cd j d1 m1 d2 m2 -> 
     at_external esemS s1 = Some (ef, sig, args1) -> 
-    Events.meminj_preserves_globals ge j -> 
+    Events.meminj_preserves_globals (Extension.ge E_S) j -> 
     inject_incr j j' -> 
     Events.inject_separated j j' m1 m2 -> 
     Mem.inject j' m1' m2' -> 
@@ -634,34 +638,34 @@ Module ExtendedSimulations. Section ExtendedSimulations.
     ACTIVE E_S s1 <> i -> 
     match_state (core_simulations i) cd j' d1 m1' d2 m2')
 
-  (make_initial_core_diagram: forall ge v1 vals1 s1 m1 v2 vals2 m2 j sig,
-    make_initial_core esemS ge v1 vals1 = Some s1 -> 
+  (make_initial_core_diagram: forall v1 vals1 s1 m1 v2 vals2 m2 j sig,
+    make_initial_core esemS (Extension.ge E_S) v1 vals1 = Some s1 -> 
     Mem.inject j m1 m2 -> 
     Forall2 (val_inject j) vals1 vals2 -> 
     Forall2 Val.has_type vals2 (sig_args sig) -> 
     exists cd, exists s2, 
-      make_initial_core esemT ge v2 vals2 = Some s2 /\
+      make_initial_core esemT (Extension.ge E_T) v2 vals2 = Some s2 /\
       match_states cd j s1 m1 s2 m2)
 
-  (safely_halted_step: forall cd j c1 m1 c2 m2 ge v1,
+  (safely_halted_step: forall cd j c1 m1 c2 m2 v1,
     match_states cd j c1 m1 c2 m2 -> 
-    safely_halted esemS ge c1 = Some v1 -> 
+    safely_halted esemS c1 = Some v1 -> 
     exists v2,
       val_inject j v1 v2 /\
-      safely_halted esemT ge c2 = Some v2 /\ 
+      safely_halted esemT c2 = Some v2 /\ 
       Mem.inject j m1 m2)
 
   (safely_halted_diagram: forall cd j m1 m1' m2 rv s1 s2 s1' c1 c2,
     match_states cd j s1 m1 s2 m2 -> 
     PROJ_CORE E_S (ACTIVE E_S s1) s1 = Some c1 -> 
     PROJ_CORE E_T (ACTIVE E_S s1) s2 = Some c2 -> 
-    safely_halted (csemS (ACTIVE E_S s1)) ge c1 = Some rv -> 
-    corestep esemS ge s1 m1 s1' m1' ->  
-    safely_halted (csemT (ACTIVE E_S s1)) ge c2 = Some rv /\
+    safely_halted (csemS (ACTIVE E_S s1)) c1 = Some rv -> 
+    corestep esemS (Extension.ge E_S) s1 m1 s1' m1' ->  
+    safely_halted (csemT (ACTIVE E_S s1)) c2 = Some rv /\
     exists s2', exists m2', exists cd', exists j', 
       inject_incr j j' /\
       Events.inject_separated j j' m1 m2 /\
-      corestep esemT ge s2 m2 s2' m2' /\
+      corestep esemT (Extension.ge E_T) s2 m2 s2' m2' /\
       match_states cd' j' s1' m1' s2' m2'),
   internal_compilability_invariant.
 
@@ -670,8 +674,9 @@ Module ExtendedSimulations. Section ExtendedSimulations.
   (core_compatS: core_compatible E_S) (core_compatT: core_compatible E_T).
 
 Program Definition extended_simulation: 
-  Forward_simulation_inject dS dT esemS esemT ge ge entry_points :=
-      Build_Forward_simulation_inject 
+  Forward_simulation_inject dS dT esemS esemT 
+      (Extension.ge E_S) (Extension.ge E_T) entry_points :=
+     Build_Forward_simulation_inject 
       core_datas match_states core_ords _ _ _ _ _ _.
 Next Obligation. apply core_ords_wf. Qed.
 Next Obligation. 
@@ -679,21 +684,22 @@ rename H0 into MATCH.
 generalize MATCH as MATCH'; intro.
 destruct MATCH as [ACT [RUN MATCH_CORES]].
 rename H into STEP.
-case_eq (RUNNABLE E_S ge st1).
+case_eq (RUNNABLE E_S st1).
 
 (*Case 1: runnable thread, appeal to core diagram for cores*)
 intros RUN1.
-assert (RUN2: RUNNABLE E_T ge st2 = true) by (rewrite <-RUN; auto).
+assert (RUN2: RUNNABLE E_T st2 = true) by (rewrite <-RUN; auto).
 destruct (active_proj_core E_S st1) as [c1 PROJ1].
-assert (exists c1', corestep (csemS (ACTIVE E_S st1)) ge c1 m1 c1' m1') as [c1' STEP1].
+assert (exists c1', corestep (csemS (ACTIVE E_S st1)) (GENV_MAP E_S (ACTIVE E_S st1)) 
+         c1 m1 c1' m1') as [c1' STEP1].
  inv esig_compilable.
  inv core_compatS.
- specialize (runnable_corestep ge st1 m1 st1' m1' c1 (csemS (ACTIVE E_S st1))).
+ specialize (runnable_corestep st1 m1 st1' m1' c1 (csemS (ACTIVE E_S st1))).
  destruct runnable_corestep as [c1' [H3 H4]]; auto.
  solve[exists c1'; auto].
 assert (PROJ1': PROJ_CORE E_S (ACTIVE E_S st1) st1' = Some c1').
  inv core_compatS.
- specialize (corestep_pres ge st1 c1 m1 c1' st1' m1' (csemS (ACTIVE E_S st1))).
+ specialize (corestep_pres st1 c1 m1 c1' st1' m1' (csemS (ACTIVE E_S st1))).
  spec corestep_pres; auto.
  spec corestep_pres; auto.
  spec corestep_pres; auto.
@@ -701,7 +707,7 @@ assert (PROJ1': PROJ_CORE E_S (ACTIVE E_S st1) st1' = Some c1').
  solve[destruct corestep_pres; auto].
 assert (ACT1': ACTIVE E_S st1 = ACTIVE E_S st1').
  inv core_compatS.
- specialize (corestep_pres ge st1 c1 m1 c1' st1' m1' (csemS (ACTIVE E_S st1))).
+ specialize (corestep_pres st1 c1 m1 c1' st1' m1' (csemS (ACTIVE E_S st1))).
  spec corestep_pres; auto.
  spec corestep_pres; auto.
  spec corestep_pres; auto.
@@ -717,7 +723,7 @@ destruct STEP2 as [STEP2|STEP2].
 (*corestep_plus case*)
 destruct STEP2 as [n STEP2].
 generalize (corestep_stepN core_compatT) as CSTEPN; intro.
-specialize (CSTEPN (S n) ge st2). 
+specialize (CSTEPN (S n) st2). 
 rewrite <-ACT in *.
 specialize (CSTEPN c2 m2 c2' m2' (csemT (ACTIVE E_S st1))).
 spec CSTEPN; auto.
@@ -759,7 +765,7 @@ split; auto.
   intros NEQ _.
   assert (_PROJ1: PROJ_CORE E_S i st1 = Some _c). 
    inv core_compatS.
-   specialize (corestep_others_forward ge st1 st1'). 
+   specialize (corestep_others_forward st1 st1'). 
    forget (ACTIVE E_S st1) as x.
    forget (ACTIVE E_T st2) as y.
    forget (ACTIVE E_S st1') as x'.
@@ -777,7 +783,7 @@ split; auto.
    solve[exists _d; auto].
   assert (_PROJ2': PROJ_CORE E_T i st2' = Some _d). 
    inv core_compatT.
-   specialize (corestep_others_backward ge st2). 
+   specialize (corestep_others_backward st2). 
    forget (ACTIVE E_S st1) as x.
    forget (ACTIVE E_T st2) as y.
    forget (ACTIVE E_S st1') as x'.
@@ -802,7 +808,7 @@ split; auto.
 (*corestep_star case*)
 destruct STEP2 as [[n STEP2] ORD].
 generalize (corestep_stepN core_compatT) as CSTEPN; intro.
-specialize (CSTEPN n ge st2). 
+specialize (CSTEPN n st2). 
 rewrite <-ACT in *.
 specialize (CSTEPN c2 m2 c2' m2' (csemT (ACTIVE E_S st1))).
 spec CSTEPN; auto.
@@ -843,7 +849,7 @@ split; auto.
   intros NEQ _.
   assert (_PROJ1: PROJ_CORE E_S i st1 = Some _c). 
    inv core_compatS.
-   specialize (corestep_others_forward ge st1 st1'). 
+   specialize (corestep_others_forward st1 st1'). 
    forget (ACTIVE E_S st1) as x.
    forget (ACTIVE E_T st2) as y.
    forget (ACTIVE E_S st1') as x'.
@@ -861,7 +867,7 @@ split; auto.
    solve[exists _d; auto].
   assert (_PROJ2': PROJ_CORE E_T i st2' = Some _d). 
    inv core_compatT.
-   specialize (corestep_others_backward ge st2). 
+   specialize (corestep_others_backward st2). 
    forget (ACTIVE E_S st1) as x.
    forget (ACTIVE E_T st2) as y.
    forget (ACTIVE E_S st1') as x'.
@@ -890,7 +896,7 @@ destruct (active_proj_core E_S) with (s := st1) as [c1 PROJ1].
 generalize PROJ1 as _PROJ1; intro.
 destruct (active_csem E_S) with (s := st1) as [CS ACT1]; inv ACT1.
 apply (runnable_false E_S) with 
- (c := c1) (CS := (csemS (ACTIVE E_S st1))) (ge := ge) in PROJ1; auto.
+ (c := c1) (CS := (csemS (ACTIVE E_S st1))) in PROJ1; auto.
 destruct PROJ1 as [[rv HALT]|[ef [sig [args AT_EXT]]]].
 
 (*active thread is safely halted*)
@@ -913,6 +919,7 @@ destruct (core_at_external (core_simulations (ACTIVE E_S st1)) (cd (ACTIVE E_S s
  as [H6 [H7 [vals2 [H8 [H9 H10]]]]].
 inv esig_compilable. 
 edestruct extension_diagram as [s2' H11]; eauto.
+admit. (*TODO: Events.*)
 destruct H11 as [m2' [cd' [j' [? [? [? ?]]]]]].
 exists s2'; exists m2'; exists cd'; exists j'.
 split3; auto; split; auto.
@@ -922,11 +929,13 @@ Qed.
 (*we punt in the make_initial_core case of the simulation proof; to do more requires 
    assuming too much about the structure of the extension w/r/t its inner cores*)
 Next Obligation. 
-inv esig_compilable; eapply make_initial_core_diagram; eauto.
+inv esig_compilable. 
+eapply make_initial_core_diagram; eauto.
 Qed.
 
 Next Obligation. 
-inv esig_compilable; eapply safely_halted_step; eauto.
+inv esig_compilable. 
+eapply safely_halted_step; eauto.
 Qed.
 
 Next Obligation. 
@@ -944,12 +953,12 @@ destruct (core_at_external (core_simulations (ACTIVE E_S st1))
             (cd (ACTIVE E_S st1)) j c1 m1 c2 m2 e vals1 ef_sig MATCH12 AT_EXT1)
  as [INJ [GLOBS [vals2 [VALINJ [TYPE AT_EXT2]]]]].
 split3; auto.
+admit. (*Events*)
 exists vals2.
 split3; auto.
 inv esig_compilable.
-specialize (at_external_match st1 m1 st2 c1 c2 m2 e ef_sig vals1 vals2 
-             (cd (ACTIVE E_S st1)) j).
-spec at_external_match; auto.
+eapply at_external_match; eauto.
+admit. (*Events*)
 Qed.
 
 Next Obligation. 
@@ -969,6 +978,8 @@ destruct (core_after_external (core_simulations (ACTIVE E_S st1))
                 (cd (ACTIVE E_S st1)) j j' c1 c2 m1 e 
                 vals1 ret1 m1' m2 m2' ret2 ef_sig)
  as [cd' [c1' [c2' [AFTER1 [AFTER2 MATCH12']]]]]; auto.
+
+admit. (*Events*)
 
 exists (core_datas_upd (ACTIVE E_S st1) cd' cd).
 assert (exists st1', after_external esemS (Some ret1) st1 = Some st1' /\
@@ -1034,7 +1045,7 @@ Qed.
 
 Lemma RGsimulations_invariant: 
   (forall i:nat, RelyGuaranteeSimulation.Sig (core_simulations i)) -> 
-  CompilabilityInvariant.Sig csemS csemT E_S E_T core_simulations match_states -> 
+  CompilabilityInvariant.Sig fS fT vS vT csemS csemT E_S E_T core_simulations match_states -> 
   internal_compilability_invariant.
 Proof.
 intro core_simulations_RGinject.
@@ -1050,25 +1061,28 @@ destruct (MATCH_INNER i d1 PROJD1) as [_d2 [_PROJD2 MATCHD]].
 rewrite _PROJD2 in PROJD2; inv PROJD2.
 forget (Extension.active E_T s2) as k.
 destruct (core_simulations_RGinject k) as [_ GUARANTEE].
-specialize (GUARANTEE ge ge (cd k) cd' m1 m1' j j' m2 m2' c1 c2 c1' c2' n).
+specialize (GUARANTEE (Extension.genv_map E_S k) (Extension.genv_map E_T k) 
+            (cd k) m1 m1' j m2 m2' c1 c2 c1' c2' n).
 intros HSTEP HMATCH.
 spec GUARANTEE; auto.
 spec GUARANTEE; auto.
+admit. (*Events: meminj_preserves_globals*)
 spec GUARANTEE; auto.
 spec GUARANTEE; auto.
 spec GUARANTEE; auto.
-spec GUARANTEE; auto.
-destruct GUARANTEE as [H1 [H2 [H3 [H4 H5]]]].
+destruct GUARANTEE as [H1 H2].
 destruct (core_simulations_RGinject i) as [RELY _].
-specialize (RELY ge (cd i) m1 m1' j j' m2 m2' d1 d2).
-spec RELY; auto.
+specialize (RELY (Extension.genv_map E_S i) (cd i) m1 m1' j j' m2 m2' d1 d2).
+apply RELY; auto.
+admit. (*Events: meminj_preserves_globals*)
+admit. (*Mem.inject j' m1' m2'; either we don't assume or we guarantee*)
 
 (*2*)
 intros until j'; intros MATCH EXT1 PRES INCR SEP INJ INJARGS FORW1 UNCH1 FORW2 UNCH2.
 intros TYS AFTER1 AFTER2 PROJ1 PROJ2 NEQ.
 forget (Extension.active E_S s1) as k.
 destruct (core_simulations_RGinject i) as [RELY _].
-specialize (RELY ge cd m1 m1' j j' m2 m2' d1 d2).
+specialize (RELY (Extension.genv_map E_S i) cd m1 m1' j j' m2 m2' d1 d2).
 apply RELY; auto.
 admit. (*Mem.inject*)
 admit. (*Events vs. Events2*)
@@ -1082,6 +1096,7 @@ Module CompilableExtension. Section CompilableExtension.
  Variables
   (F V: Type) (** global environments *)
   (xS xT: Type) (** corestates of source and target extended semantics *)
+  (fS fT vS vT: nat -> Type) (** global environments of core semantics *)
   (cS cT: nat -> Type) (** corestates of source and target core semantics *)
   (dS dT: Type) (** initialization data *)
   (Z: Type) (** external states *)
@@ -1089,33 +1104,51 @@ Module CompilableExtension. Section CompilableExtension.
   (Zext: Type) (** portion of Z external to extension *)
   (esemS: CoreSemantics (Genv.t F V) xS mem dS) (** extended source semantics *)
   (esemT: CoreSemantics (Genv.t F V) xT mem dT) (** extended target semantics *)
-  (csemS: forall i:nat, CoreSemantics (Genv.t F V) (cS i) mem dS) (** a set of core semantics *)
-  (csemT: forall i:nat, CoreSemantics (Genv.t F V) (cT i) mem dT) (** a set of core semantics *)
+  (csemS: forall i:nat, CoreSemantics (Genv.t (fS i) (vS i)) (cS i) mem dS) (** a set of core semantics *)
+  (csemT: forall i:nat, CoreSemantics (Genv.t (fT i) (vT i)) (cT i) mem dT) (** a set of core semantics *)
   (csig: ext_sig mem Z) (** client signature *)
   (esig: ext_sig mem Zext) (** extension signature *)
   (handled: list AST.external_function). (** functions handled by this extension *)
 
- Variable (E_S: Extension.Sig cS Zint esemS (fun i:nat => Some (csemS i)) csig esig handled).
- Variable (E_T: Extension.Sig cT Zint esemT (fun i:nat => Some (csemT i)) csig esig handled).
+ Variable (E_S: Extension.Sig (fun i => Genv.t (fS i) (vS i)) cS Zint esemS 
+                  (fun i:nat => Some (csemS i)) csig esig handled).
+ Variable (E_T: Extension.Sig (fun i => Genv.t (fT i) (vT i)) cT Zint esemT 
+                  (fun i:nat => Some (csemT i)) csig esig handled).
 
  Variable ge: Genv.t F V.
  Variable entry_points: list (val*val*signature).
 
+ Notation GENV_MAP := (Extension.genv_map).
+ Notation PROJ_CORE := (Extension.proj_core).
+ Infix "\o" := (Extension.zmult) (at level 66, left associativity). 
+ Notation ACTIVE := (Extension.active).
+ Notation RUNNABLE := (Extension.runnable).
+ Notation "'CORE' i 'is' ( CS , c ) 'in' s" := 
+   (csem i = Some CS /\ PROJ_CORE i s = Some c)
+   (at level 66, no associativity, only parsing).
+ Notation core_exists := (Extension.core_exists).
+ Notation active_csem := (Extension.active_csem).
+ Notation active_proj_core := (Extension.active_proj_core).
+ Notation notat_external_handled := (Extension.notat_external_handled).
+ Notation at_external_not_handled := (Extension.at_external_not_handled).
+ Notation ext_upd_at_external := (Extension.ext_upd_at_external).
+ Notation runnable_false := (Extension.runnable_false).
+
  Import Sim_inj.
-
- Variable core_simulations: forall i:nat, 
-   Forward_simulation_inject dS dT (csemS i) (csemT i) ge ge entry_points.
-
- Variable core_compatibleS: core_compatible E_S.
- Variable core_compatibleT: core_compatible E_T.
 
  Variable max_threads: nat.
 
- Lemma ExtensionCompilability: CompilableExtension.Sig csemS csemT E_S E_T core_simulations.
+ Variable core_simulations: forall i:nat, 
+   Forward_simulation_inject dS dT (csemS i) (csemT i) 
+     (GENV_MAP E_S i) (GENV_MAP E_T i) entry_points.
+
+ Lemma ExtensionCompilability: 
+   CompilableExtension.Sig fS fT vS vT csemS csemT E_S E_T core_simulations.
  Proof.
  eapply (CompilableExtension.Make 
-  (ExtendedSimulations.core_ords cS cT csemS csemT core_simulations max_threads)).
- intros H1 H2.
+  (ExtendedSimulations.core_ords fS fT vS vT csemS csemT E_S E_T 
+    core_simulations max_threads)).
+ intros H1 H2 H3 H4.
  eapply ExtendedSimulations.extended_simulation; eauto.
  eapply ExtendedSimulations.RGsimulations_invariant; eauto.
  Qed.
